\pagebreak\section*{Задача 1114}
Найти общее решение дифференциального уравнения: $$ x^2y'' + 2xy' - (x^2 + 2x + 2)y = 0. $$
\begin{solution}
    1) При $ x_0 = 0, p_0(0) = 0 $ => Общий случай $ y = \sum_{k = 0}^{+\infty} y_k x^{k + \alpha} $
    $$ \sum_{k = 0}^{\infty} (k + \alpha)(k + \alpha - 1) x^{k + \alpha - 2 + 2} y_k + 2 \sum_{k = 0}^{\infty} (x + \alpha) x^{k + \alpha - 1 + 1} y_k - \sum_{k = 0}^{\infty} x^{k + \alpha + 2} y_k - 2 \sum_{k = 0}^{\infty} x^{k + \alpha + 1} y_k - 2 \sum_{k = 0}^{\infty} x^{k + \alpha} y_k, $$ 
    min степень икса: $ k + \alpha, k_{min} = 0 $ => $\alpha$ \par
    2) По $ x^{\alpha}: $ $$ y_0 (\alpha (\alpha - 1) + 2\alpha - 2) $$
    $$ \alpha (\alpha - 1) + 2\alpha - 2 = 0 $$
    $$ \alpha^2 + \alpha - 2 = 0 => \alpha_1 = -2, \alpha_2 = 1. $$
    3) Рассмотрим $\alpha = 1:$
    $$ \sum_{k = 0}^{\infty} \underset{k = p - 1}{(k + 1) k y_k x^{k + 1}} + 2 \sum_{k = 0}^{\infty} \underset{k = p - 1}{(k + 1) y_k x^{k + 1}} - \sum_{k = 0}^{\infty} \underset{k = p - 3}{y_k x^{k + 3}} - 2 \sum_{k = 0}^{\infty} \underset{k = p - 2}{y_k x^{k + 2}} - 2 \sum_{k = 0}^{\infty} \underset{k = p - 1}{y_k x^{k + 1}} $$
    По $x^p: $ $$ p (p - 1) y_{p - 1} + 2 p y_{p - 1} - y_{p - 3} - 2y_{p - 2} = 0 $$
    $$ (p^2 + p - 2) y_{p - 1} = y_{p - 3} + 2y_{p - 2} $$
    $$ y_{p - 1} = \dfrac{y_{p - 3} + 2y_{p - 2}}{p^2 + p -2} $$
    4) Построим матрицу: 
    $
        \begin{array}{ccc}
                  & 1. & 2. \\
            y_0 = & 1  & 0  \\
            y_1 = & 0  & 1  \\
        \end{array}
    $ \par
    1. $ p = 2, y_1 = \dfrac{0 + 2 * 1}{4} = \dfrac{1}{2} $ \par
       \quad$ p = 3, y_2 = \dfrac{1 + 2 *0}{10} = \dfrac{1}{10} $ \par
       \quad$ p = 4, y_3 = \dfrac{1}{2} $ \par
    2. $ p = 2, y_1 = 0 $ \par
       \quad$ p = 3, y_2 = \dfrac{2}{10} $ \par
       \quad$ p = 4, y_3 = \dfrac{0 + \dfrac{4}{10}}{18} = \dfrac{1}{45} $ \par
    
    5) $y_1 = $

\end{solution}\pagebreak