\section*{Номер 1145}
$$ \begin{cases}
        2zy' = y^2 - z^2 + 1 \\
        z' = z + y
    \end{cases} $$

\begin{solution}
    $$
        \begin{cases}
            2z(z' - z)' = (z' - z)^2 - z^2 + 1 \\
            y = z' - z
        \end{cases}
    $$
    $$ 2zz'' - 2zz' = (z')^2 - 2z'z + z^2 - z^2 + 1 $$
    $$ 2zz'' - (z')^2 - 1 = 0 \text{ - понизить порядок. } $$
    Нет явно заданного аргумента => замена $ z' = p(z); z'' = p_z'\cdot p $
    $$ 2z \cdot p'p - p^2 - 1 = 0 $$
    $$ 2z \cdot \dfrac{dp}{dz} \cdot p = p^2 + 1 = 0 | \cdot \dfrac{dz}{(p^2 + 1) \cdot 2z} $$
    $$ \int \dfrac{p}{p^2 + 1} dp = \int \dfrac{dz}{2z} = 0 $$
    Пусть $ t = p^2 + 1 $, $ t' = 2p $. Тогда: $ dp = \dfrac{1}{t'} dt => dp = \dfrac{1}{2p} dt $.
    $$ \int \dfrac{p}{p^2 + 1} dp = \int \dfrac{p}{2p \cdot t} dt = \dfrac{1}{2} \int \dfrac{dt}{t} = \dfrac{1}{2} \ln |t| $$
    $$ \dfrac{1}{2} \ln |p^2 + 1| = \dfrac{1}{2} \ln |z| - C $$
    $$ e^{\ln |p^2 + 1|} = e^{\ln |z| - C} $$
    $$ p^2 + 1 = \dfrac{z}{C_1} $$
    $$ p = \pm \sqrt{\dfrac{z}{C_1} - 1} $$
    $$ \dfrac{dz}{dx} = \pm \sqrt{\dfrac{z}{C_1} - 1} $$
    $$ \pm \int \dfrac{dz}{\sqrt{\dfrac{z}{C_1} - 1}} = \int dx $$
    $$ \pm 2 \sqrt{C_1 z - C_1^2} + C_2 = x + C_3 \text{ => } $$
    => $ z = C_1 + \dfrac{1}{4 C_1} (x + C_2)^2 $ => \par
    \textbf{Ответ: $ y = z' - z = \dfrac{1}{C_2} (x + C_2) - \dfrac{1}{4 C_1} (x + C_2)^2 - C_1 $}

\end{solution}\pagebreak