\section*{Номер 1201}

$$ z \cdot \dfrac{\delta z}{\delta x} - xy \cdot \dfrac{\delta z}{\delta y} = 2xz; \quad x + y = 2; \quad yz = 1 $$

\begin{solution}
    $$ \dfrac{dx}{z} = \dfrac{dy}{-xy} = \dfrac{dz}{2xz} $$

    \begin{itemize}
        \item
              $$ \dfrac{dy}{-xy} = \dfrac{dz}{2xz}\quad=>\quad -2\int \dfrac{dy}{y} = \int \dfrac{dz}{z}; $$
              $$ e^{\ln |z| + \ln |y|^2} = e^{C_1} $$
              $$ y^2 z = C_1 $$
        \item
              $$ \dfrac{dx}{z} = \dfrac{dz}{2xz} \quad=>\quad \int 2xdx = \int dz; \quad x^2 + C_2 = z $$
              С учетом заданных доп. условий:
              $$
                  \begin{cases}
                      C_1 = y^2 z = yz \cdot y = y                    \\
                      C_2 = x^2 - z = (2 - y)^2 - z = (2 - C_1)^2 - z \\
                      x + y = 2 \quad=>\quad x = 2 - y                \\
                      yz = 1                                          \\
                  \end{cases}
              $$
    \end{itemize}
    \textbf{Ответ: $ (2 - y^2 z)^2 = x^2 $}
\end{solution}\pagebreak