\section*{Номер 770}

$$ xy'' - y' = 0 $$
$$ y'(1) = 0, \quad y(2) = 0 $$

\begin{solution}
    Обозначим $ z = y' $, тогда уравнение принимает вид:
    $$ xz' - z = 0 $$
    Решаем уравнение:

    $$ xz' = z $$
    $$ \dfrac{dz}{z} = \dfrac{dx}{x} $$
    $$ \ln |z| = \ln |x| + C $$

    $$ z = Cx $$

    $$ y' = Cx $$
    $$ y = \dfrac{Cx^2}{2} + C_1 $$
    Рассмотрим области $ 1 \leq x \leq s $:
    $$ G(x,s) = A(s) \dfrac{x^2}{2} + B(s) $$
    $$ G'(x,s) = A(s) x $$
    Так как $ G'(1,s) = 0 $, то:
    $$ A(s) = 0 $$
    $$ G(x,s) = B(s) $$
    Рассмотрим область $ s \leq x \leq 2 $:
    $$ G(x,s) = C(s) \dfrac{x^2}{2} + D(s) $$
    $$ C(s) \dfrac{2^2}{2} + D(s) = 0 $$
    $$ D(s) = -2C(s) $$
    $$ G(x,s) = C(s) \left( \dfrac{x^2}{2} - 2 \right) $$
    $$ G(s+0, s) - G(s-0, s) = 1 $$
    $$ C(s) s - 0 = 1 $$
    $$ C(s) = \dfrac{1}{s} $$

\end{solution}\pagebreak

