\section*{Задача 1110}
Найти общее решение дифференциального уравнения:
$$ xy'' + 2y' + xy = 0 $$
\begin{solution}
    1) При $x_0 = 0 $ : $ p_0(0) = 0 $ => $ \sum_{k = 0}^{\infty} y_k x^{k + \alpha} $ \par
    2) Преобразуем: $$ \sum_{k = 0}^{\infty} y_k (k + \alpha) (k + \alpha - 1) x^{k + \alpha - 2 + 1} + 2 \sum_{k = 0}^{\infty} y_k (k + \alpha) x^{k + \alpha - 1} + \sum_{k = 0}^{\infty} y_k x^{k + \alpha + 1} = 0 $$
    3) min степень $x$: $ k + \alpha - 1 $, $ k = 0 $ => $ \alpha - 1 $ => \par
    при $ k = 0 $: $ y_0 \alpha (\alpha - 1) x^{\alpha - 1} + 2 y_0 \alpha x^{\alpha - 1} + y_0 x^{\alpha + 1} $ \par
    $ y_0 (\alpha (\alpha - 1) + 2 \alpha) $, где $ (\alpha (\alpha - 1) + 2 \alpha) = 0 $, при $ x^{\alpha - 1} $ (минимальная степень $x$) \par
    $ \alpha (\alpha + 1) = 0 $ => $ \alpha = 0 $; $-1$, но берем $-1$, т.к. $\alpha = 0$ делает ряд обычным. \par
    4) Получаем ряд: $$ \sum_{k = 0}^{\infty} \underset{k = p + 2}{y_k (k - 1) (k - 2) x^{k - 2}} + 2 \sum_{k = 0}^{\infty} \underset{k = p + 2}{y_k (k - 1) x^{k - 2}} + \sum_{k = 0}^{\infty} \underset{k = p}{y_k x^k = 0} $$
    5) При $ x^p $ : $$ y_{p + 2} (p + 1) + 2y_{p + 2} (p + 1) + y_p = 0 $$
    $$ y_{p + 2} (p + 1) (p + 2) + y_p = 0 $$
    $$ y_{p + 2} = -\dfrac{y_p}{(p + 1) (p + 2)} $$
    6) Построим матрицу: 
    $
        \begin{array}{ccc}
                  & 1) & 2) \\
            y_0 = & 1  & 0  \\
            y_1 = & 0  & 1  \\
        \end{array}
    $ \par
    \quad1) $ y_2 = -\dfrac{1}{2} = -\dfrac{1}{2!} $, $ y_3 = 0 $, $ y_4 = -\dfrac{-\dfrac{1}{2}}{3 \cdot 4} = \dfrac{1}{24} = \dfrac{1}{4!} $, $\cdots$ => \par
    => $ y_1 = \dfrac{1}{x} - \dfrac{x}{2!} + \dfrac{x^3}{4!} - \dfrac{x^5}{6!} + \cdots $\par
    \quad2) $ y_2 = 0 $, $ y_3 = -\dfrac{1}{1 \cdot 2 \cdot 3} = -\dfrac{1}{3!} $, $ y_4 = 0 $, $\cdots$ => \par
    => $ y_2 = 1 - \dfrac{x^2}{3!} + \dfrac{x^4}{5!} - \dfrac{x^6}{7!} + \cdots $ \par
    7) Общее решение будет выглядить так: $ y = c_1y_1 + c_2y_2 $
\end{solution}\pagebreak
