\section*{Номер 1163}
$$ \dfrac{dx}{y} = - \dfrac{dy}{x} = \dfrac{dz}{u} = - \dfrac{du}{z} $$

\begin{solution}
    Пусть $ \phi = yz - ux $. Тогда:
    $$ \dfrac{\delta \phi}{\delta y} = z; \dfrac{\delta \phi}{\delta z} = y; \dfrac{\delta \phi}{\delta u} = -x; \dfrac{\delta \phi}{\delta x} = -u $$
    Проверить, чтобы $ \dfrac{\delta \phi}{\delta x} \cdot F_x + \dfrac{\delta \phi}{\delta y} \cdot F_y + \dfrac{\delta \phi}{\delta z} \cdot F_z + \dfrac{\delta \phi}{\delta u} \cdot F_u = 0 $
    $$ \dfrac{dx}{y} = - \dfrac{dy}{x} => F_x = y; F_y = -x $$
    $$ \dfrac{dz}{u} = - \dfrac{du}{z} => F_u = -z; F_z = u $$
    Имеем: $ -u \cdot y + z \cdot (-x) + y \cdot u + (-x) \cdot (-z) = 0 $
    $$ 0 = 0 \text{ => $\phi$ - первый $\int$-л системы} $$


\end{solution}\pagebreak