\section*{Номер 1180}
$$ (z - y)^2 \dfrac{\delta z}{\delta x} + xz \cdot \dfrac{\delta z}{\delta y} = xy $$

\begin{solution}
    $$ \dfrac{dx}{(z - y)^2} = \dfrac{dy}{xz} = \dfrac{dz}{xy} $$
    \begin{itemize}
        \item
              $$ \dfrac{dy}{xz} = \dfrac{dz}{xy};\quad \dfrac{dy}{z} = \dfrac{dz}{y};\quad \int ydy = \int zdz $$
              $$ y^2 - z^2 = C_1 $$
        \item
              $$ \dfrac{dy - dz}{x(z - y)} = \dfrac{dx}{(z - y)^2};\quad \dfrac{dy - dz}{x} = \dfrac{dx}{z - y} $$
              $$ (z - y) \cdot d(z - y) + xdx = 0 $$
              $$ d((z - y)^2 + x^2) = 0\quad => \quad (z - y)^2 + x^2 = C_2 $$
    \end{itemize}
    $$ F(y^2 - z^2, x^2 + (z - y)^2) = 0 $$

\end{solution}

\section*{Номер 1182}
$$ y \dfrac{\delta z}{\delta x} + z \dfrac{\delta z}{\delta y} = \dfrac{y}{x} $$

\begin{solution}
    $$ \dfrac{dx}{y} = \dfrac{dy}{z} = x \dfrac{dz}{y} $$
    \begin{itemize}
        \item
              $$ \dfrac{dx}{y} = \dfrac{xdz}{y};\quad \int \dfrac{dx}{x} = \int dz \quad => \quad \ln |x| = z + C_1 $$
        \item
              $$ \dfrac{dx}{y} = \dfrac{dy}{z},\quad z = \ln |x| - C_1 $$
              $$ dx \cdot (\ln |x| - C_1) = ydy $$
              $$ \int \ln |x| dx - \int C_1 dx = \int ydy $$
              $$ \int \ln |x| \cdot 1 dx = \ln x \cdot x - \int x \cdot \dfrac{1}{x} dx = \ln x \cdot x - x $$
        \item
              $$ x \cdot ln|x| - x - x C_1 = \dfrac{1}{2} y^2 + C_2 $$
              $$ -x + xz - \dfrac{1}{2} y^2 = C_2 $$
              $$ -2x + 2xz - y^2 = C_2 $$
    \end{itemize}
    $$ F(\ln|x| - z, 2x(z - 1) - y^2) = 0 $$
\end{solution}\pagebreak