\section*{Номер 212}

$$ (2x^2y^3 - 1)y dx + (4x^2y^3 - 1)x dy = 0 $$

\begin{solution}
    1) $$ (2x^2y^4 - y)_y' = (4x^3y^3 - x)_x' $$
    $$ 8x^2y^3 - 1 = 12x^2y^3 - 1 \text{ - неверно. Проверка в полных диф-ах не пройдена.} $$
    2) $$ 2x^2y^4dx - ydx + 4x^3y^3dy - xdy = 0 $$
    $$ 2x^2y^2 \cdot d(xy^2) - d(xy) = 0 $$
    Замена $$ \begin{cases}
        z = xy \Rightarrow z^2 = x^2y^2 \\
        t = xy^2
    \end{cases} $$

    $$ 2z^2 dt - dz = 0 $$
    $$ 2 \int dt - \int \dfrac{dz}{z^2} = 0 $$
    $$ 2xy^2 + \dfrac{1}{xy} = C \text{ - общее решение, а $x = 0, y = 0$ - особые точки.}$$
\end{solution}

\section*{Номер 257}
$$ (y')^2 - 2xy' = 8x^2 $$
\begin{solution}
    $$ D = 4x^2 = 36x^2 $$
    $$ y_{1,2}' = \dfrac{2x \pm 6x}{2} $$
    Общие решения: $ y_1 = 2x^2 + C \quad y_2 = -x^2 + C $
    
\end{solution}

\section*{Номер 274}

$$ y = (y' - 1) \cdot e^{y'}$$

\begin{solution}
    $$ p = y' \Rightarrow \dfrac{dy}{dx} = p \Rightarrow dx = \dfrac{dy}{p} $$
    $$ y = (p - 1) \cdot e^p $$
    $$ dx = \dfrac{dy}{p} = e^p dp $$
    $$ x = e^p + C \quad y = (p - 1) \cdot e^p \quad y = -1 $$
\end{solution}
\pagebreak